x64 crefine: prove several lemmas in Retype_C
To prove that retyping a TCB establishes the state relation for TCBs,
it is necessary to prove that the C FPU null state is always equal to
the Haskell FPU null state. This commit therefore includes some
machinery for maintaining the state relation for the FPU null state,
and repairs many proofs.

proof/crefine/X64/StateRelation_C.thy
@@ -179,16 +179,25 @@ where
            \<and> ptr_span (ioport_table_Ptr (symbol_table ''x86KSAllocatedIOPorts'')) \<subseteq> kernel_data_refs"
 
 definition
+  fpu_null_state_relation :: "heap_raw_state \<Rightarrow> bool"
+where
+  "fpu_null_state_relation hrs \<equiv>
+    clift hrs (Ptr (symbol_table ''x86KSnullFpuState''))
+      = Some (user_fpu_state_C (ARRAY i. FPUNullState (finite_index i))) \<and>
+    ptr_span (fpu_state_Ptr (symbol_table ''x86KSnullFpuState'')) \<subseteq> kernel_data_refs"
+
+definition
   carch_state_relation :: "Arch.kernel_state \<Rightarrow> globals \<Rightarrow> bool"
 where
   "carch_state_relation astate cstate \<equiv>
-  x64KSKernelVSpace astate = x64KSKernelVSpace_C \<and>
-  array_relation (op = \<circ> option_to_ptr) (2^asid_high_bits - 1) (x64KSASIDTable astate) (x86KSASIDTable_' cstate) \<and>
-  ccr3_relation (x64KSCurrentUserCR3 astate) (x64KSCurrentUserCR3_' cstate) \<and>
-  global_ioport_bitmap_relation (clift (t_hrs_' cstate)) (x64KSAllocatedIOPorts astate) \<and>
-  x64KSNumIOAPICs astate = UCAST (32 \<rightarrow> 64) (num_ioapics_' cstate) \<and>
-  array_relation x64_irq_state_relation maxIRQ (x64KSIRQState astate) (x86KSIRQState_' cstate) \<and>
-  carch_globals astate"
+    x64KSKernelVSpace astate = x64KSKernelVSpace_C \<and>
+    array_relation (op = \<circ> option_to_ptr) (2^asid_high_bits - 1) (x64KSASIDTable astate) (x86KSASIDTable_' cstate) \<and>
+    ccr3_relation (x64KSCurrentUserCR3 astate) (x64KSCurrentUserCR3_' cstate) \<and>
+    global_ioport_bitmap_relation (clift (t_hrs_' cstate)) (x64KSAllocatedIOPorts astate) \<and>
+    fpu_null_state_relation (t_hrs_' cstate) \<and>
+    x64KSNumIOAPICs astate = UCAST (32 \<rightarrow> 64) (num_ioapics_' cstate) \<and>
+    array_relation x64_irq_state_relation maxIRQ (x64KSIRQState astate) (x86KSIRQState_' cstate) \<and>
+    carch_globals astate"
 
 end
 
@@ -1121,5 +1130,10 @@ lemma (in kernel) cmap_relation_cs_atD:
   apply (drule (1) injD)
   apply simp
   done
+
+definition (in kernel)
+  rf_sr :: "(KernelStateData_H.kernel_state \<times> cstate) set"
+  where
+  "rf_sr \<equiv> {(s, s'). cstate_relation s (globals s')}"
 
 end
