proof/crefine/X64/PSpace_C.thy
@@ -130,6 +130,7 @@ lemma storePTE_Basic_ccorres':
           erule ko_at_projectKO_opt, simp+)
   apply (simp add: cready_queues_relation_def
                    carch_state_relation_def
+                   fpu_null_state_heap_update_tag_disj_simps
                    cmachine_state_relation_def
                    Let_def typ_heap_simps
                    cteCaps_of_def update_pte_map_tos bit_simps)
@@ -176,6 +177,7 @@ lemma storePDE_Basic_ccorres':
           erule ko_at_projectKO_opt, simp+)
   apply (simp add: cready_queues_relation_def
                    carch_state_relation_def
+                   fpu_null_state_heap_update_tag_disj_simps
                    cmachine_state_relation_def
                    Let_def typ_heap_simps bit_simps
                    cteCaps_of_def update_pde_map_tos)
@@ -221,6 +223,7 @@ lemma storePDPTE_Basic_ccorres':
           erule ko_at_projectKO_opt, simp+)
   apply (simp add: cready_queues_relation_def
                    carch_state_relation_def
+                   fpu_null_state_heap_update_tag_disj_simps
                    cmachine_state_relation_def
                    Let_def typ_heap_simps
                    cteCaps_of_def update_pdpte_map_tos bit_simps)
@@ -267,6 +270,7 @@ lemma storePML4E_Basic_ccorres':
           erule ko_at_projectKO_opt, simp+)
   apply (simp add: cready_queues_relation_def
                    carch_state_relation_def
+                   fpu_null_state_heap_update_tag_disj_simps
                    cmachine_state_relation_def
                    Let_def typ_heap_simps bit_simps
                    cteCaps_of_def update_pml4e_map_tos)
